kalloc/Verif_clients.v
@@ -280,6 +280,65 @@ Definition kfree_kalloc_kfree_kalloc_spec:=
                     else both_pointers_case
 ).
 
+Definition kfree_kfree_kalloc_spec :=
+    DECLARE _kfree_kfree_kalloc
+    WITH sh : share, pa1:val, pa2:val, original_freelist_pointer:val, xx:Z, gv:globals, ls : list val, next:val
+    PRE [ tptr tvoid, tptr tvoid ]
+        PROP(
+            is_pointer_or_null pa1 /\
+            is_pointer_or_null pa2 
+        ) 
+        PARAMS (pa1; pa2) GLOBALS(gv)
+        SEP (
+            KF_globals gv  sh ls xx original_freelist_pointer *
+            (if eq_dec pa1 nullval then emp
+            else (kalloc_token' KF_APD sh (sizeof t_run) pa1)) *
+            (if eq_dec pa2 nullval then emp
+            else (kalloc_token' KF_APD sh (sizeof t_run) pa2))
+        )
+    POST [ tptr tvoid ]
+        EX r,
+        PROP(
+            ((pa1 = nullval) /\ (pa2 = nullval) /\ r = original_freelist_pointer) \/
+            ((pa1 <> nullval) /\  (pa2 <> nullval) /\ r = pa2) \/
+            ((pa1 <> nullval) /\  (pa2 = nullval) /\ r = pa1) \/
+            ((pa1 = nullval) /\  (pa2 <> nullval) /\ r = pa2)
+        )
+        RETURN (r) (* we return the head like in the pop function*)
+        SEP 
+        (
+            let freelist_only_pa1_null_case :=
+                kalloc_token' KF_APD sh (sizeof t_run) pa2 *
+                KF_globals gv sh ls xx original_freelist_pointer
+            in
+            let freelist_only_pa2_null_case :=
+                kalloc_token' KF_APD sh (sizeof t_run) pa1 * 
+                KF_globals gv sh ls xx original_freelist_pointer
+            in
+            let freelist_both_null_case :=
+                if eq_dec original_freelist_pointer nullval then
+                    emp * KF_globals gv sh ls xx original_freelist_pointer
+                else
+                    (EX next, EX ls',
+                    !! (next :: ls' = ls) &&
+                    KF_globals gv sh ls' xx next *
+                    kalloc_token' KF_APD sh (sizeof t_run) original_freelist_pointer)
+            in
+            let both_pointers_case :=
+                KF_globals gv sh (original_freelist_pointer::ls) xx pa1 *
+                (*kalloc_token' KF_APD sh (sizeof t_run) pa1 *)
+                kalloc_token' KF_APD sh (sizeof t_run) pa2
+            in
+            if eq_dec pa1 nullval then
+                if eq_dec pa2 nullval then
+                    freelist_both_null_case
+                else freelist_only_pa1_null_case
+            else 
+                if eq_dec pa2 nullval then
+                    freelist_only_pa2_null_case
+                else both_pointers_case
+        ).
+
 Definition KFGprog_clients: funspecs := KFGprog ++ [kalloc_write_pipe_spec; kfree_kalloc_spec; kalloc_write_42_spec; kalloc_write_42_kfree_spec].
 
 
@@ -295,10 +354,6 @@ forward_call (kalloc_spec_sub KF_APD t_struct_pipe) (gv, sh , ls, xx, original_f
         * rewrite H in H0; auto_contradict.
         * forward. entailer.
     + Intros ab. forward_if.
-       (* *
-        rewrite mem_mgr_split. rewrite my_kalloc_token_split. Intros. rewrite kalloc_token_sz_split.
-        Intros. entailer!.*)
-        *
         rewrite mem_mgr_split. rewrite my_kalloc_token_split. Intros. rewrite kalloc_token_sz_split.
         Intros. 
         rewrite memory_block_data_at_; auto. rewrite data_at__eq. Intros. forward.
@@ -371,10 +426,10 @@ Proof.
         rewrite memory_block_data_at_; auto. rewrite data_at__eq. Intros. forward.
         forward. 
         forward_call (kfree_spec_sub KF_APD tint) (original_freelist_pointer, gv, sh , snd ab, xx, (fst ab)). (* call kfree *)
-        -- if_tac; auto_contradict.
+        -- if_tac_auto_contradict.
             unfold my_kalloc_token. rewrite kalloc_token_sz_split. entailer!.
             sep_apply data_at_memory_block. entailer!.
-        -- if_tac; auto_contradict.
+        -- if_tac_auto_contradict.
             forward. Exists (Vint (Int.repr 42)).
             unfold KF_globals.
             inversion H0. rewrite H9; rewrite H10.
@@ -392,46 +447,46 @@ forward_call (gv, sh, pa1, original_freelist_pointer, xx, ls).
     + if_tac.
         * if_tac.
             -- forward_call (gv, sh, pa2, original_freelist_pointer, xx, ls).
-                ++ if_tac; auto_contradict.
+                ++ if_tac_auto_contradict.
                     entailer!.
-                ++ if_tac; auto_contradict. Intros vret0.
-                    if_tac; auto_contradict.
+                ++ if_tac_auto_contradict. Intros vret0.
+                    if_tac_auto_contradict.
                     forward.
                     Exists vret0. entailer!.
                     destruct H6 as [ [H11 [H12 H13]] | [[H21 H22] | [H31 [H32 H33]]] ]; auto.
             --forward_call (gv, sh, pa2, original_freelist_pointer, xx, ls).
-                ++ if_tac; auto_contradict. entailer!.
-                ++ if_tac; auto_contradict. Intros vret0. forward.
+                ++ if_tac_auto_contradict. entailer!.
+                ++ if_tac_auto_contradict. Intros vret0. forward.
                   Exists vret0. entailer!.
                   destruct H6 as [ [H11 [H12 H13]] | [[H21 H22] | [H31 [H32 H33]]] ]; auto_contradict. do 4 right. left. auto.
         * if_tac; Intros ab.
             -- destruct ls as [ | next1 ls1]; auto_contradict. (*unfold abbreviate in POSTCONDITION.*)
                 forward_call (gv, sh, pa2, next1, xx, ls1).
-                ++ if_tac; auto_contradict.
+                ++ if_tac_auto_contradict.
                 inversion H5. rewrite H8; rewrite H9. entailer!.
-                ++ if_tac; auto_contradict. if_tac; auto_contradict. 
+                ++ if_tac_auto_contradict. if_tac_auto_contradict. 
                     ** Intros vret0. forward.
-                    Exists vret0. Exists nullval ls1. if_tac; auto_contradict. entailer!.
+                    Exists vret0. Exists nullval ls1. if_tac_auto_contradict. entailer!.
                     destruct H8 as [ [H11 [H12 H13]] | [[H21 H22] | [H31 [H32 H33]]] ]; auto_contradict. 
                     do 5 right. split; auto.
                     ** Intros vret0. Intros ab0. forward.
-                    Exists vret0. Exists (next1) (snd ab). if_tac; auto_contradict.
+                    Exists vret0. Exists (next1) (snd ab). if_tac_auto_contradict.
                     Exists (fst ab0) (snd ab0). entailer!.
                     do 5 right. split; auto.
             -- destruct ls as [ | next1 ls1]; auto_contradict. 
                 forward_call (gv, sh, pa2, next1, xx, ls1).
-                ++ if_tac; auto_contradict.
+                ++ if_tac_auto_contradict.
                 inversion H5. rewrite H8; rewrite H9. entailer!.
-                ++ Intros vret0. forward. if_tac; auto_contradict.
+                ++ Intros vret0. forward. if_tac_auto_contradict.
                 Exists vret0. Exists next1 ls1. entailer!.
                 destruct H6 as [ [H11 [H12 H13]] | [[H21 H22] | [H31 [H32 H33]]] ]; auto_contradict. 
                 do 4 right. left; split; auto.
     + if_tac.
         -- forward_call (gv, sh, pa2, original_freelist_pointer, xx, ls).
-            ++ if_tac; auto_contradict.
+            ++ if_tac_auto_contradict.
                 entailer!.
-            ++ if_tac; auto_contradict. Intros vret0.
-                if_tac; auto_contradict.
+            ++ if_tac_auto_contradict. Intros vret0.
+                if_tac_auto_contradict.
                 ** forward. 
                 Exists vret0. entailer!.
                 destruct H5 as [ [H11 [H12 H13]] | [[H21 H22] | [H31 [H32 H33]]] ]; auto.
@@ -442,8 +497,8 @@ forward_call (gv, sh, pa1, original_freelist_pointer, xx, ls).
                     do 2 right. left; split; auto.
                     do 3 right. left; split; auto.
         -- Intros. forward_call (gv, sh, pa2, original_freelist_pointer, xx, ls).
-            ++ if_tac; auto_contradict. entailer!.
-            ++ if_tac; auto_contradict. 
+            ++ if_tac_auto_contradict. entailer!.
+            ++ if_tac_auto_contradict. 
                 Intros vret0. forward.
                 Exists vret0. entailer!.
                 destruct H5 as [ [H11 [H12 H13]] | [[H21 H22] | [H31 [H32 H33]]] ]; auto_contradict.
@@ -456,34 +511,34 @@ Proof.
 start_function. Intros.
 if_tac; if_tac; destruct H; 
 forward_call (kfree_spec_sub KF_APD t_run) (pa1, gv, sh , ls, xx, original_freelist_pointer). (* call kfree *)
-- if_tac; auto_contradict. unfold KF_globals. entailer!.
+- if_tac_auto_contradict. unfold KF_globals. entailer!.
 - forward_call (kalloc_spec_sub KF_APD t_run) (gv, sh , ls, xx, original_freelist_pointer). (* kalloc *)
-    + if_tac; auto_contradict. entailer!.
-    + if_tac; auto_contradict. 
+    + if_tac_auto_contradict. entailer!.
+    + if_tac_auto_contradict. 
         * forward_call (kfree_spec_sub KF_APD t_run) (pa2, gv, sh , ls, xx, original_freelist_pointer). (* call kfree *)
-            -- if_tac; auto_contradict. entailer!.
-            -- if_tac; auto_contradict. forward_call (kalloc_spec_sub KF_APD t_run) (gv, sh , ls, xx, original_freelist_pointer). (* kalloc *)
+            -- if_tac_auto_contradict. entailer!.
+            -- if_tac_auto_contradict. forward_call (kalloc_spec_sub KF_APD t_run) (gv, sh , ls, xx, original_freelist_pointer). (* kalloc *)
                 if_tac.
                     ++ forward. Exists nullval; unfold KF_globals. entailer!.
                     ++ Intros ab. destruct ls; auto_contradict.
         * Intros ab. destruct ls; auto_contradict. 
         forward_call (kfree_spec_sub KF_APD t_run) (pa2, gv, sh , snd ab, xx, fst ab). (* call kfree *)
             -- entailer!.
-            -- if_tac; auto_contradict. forward_call (kalloc_spec_sub KF_APD t_run) (gv, sh , snd ab, xx, fst ab). (* kalloc *)
+            -- if_tac_auto_contradict. forward_call (kalloc_spec_sub KF_APD t_run) (gv, sh , snd ab, xx, fst ab). (* kalloc *)
                 if_tac.
                     ++ forward. Exists (fst ab) (fst ab) (snd ab). if_tac.
                         ** unfold KF_globals. unfold my_kalloc_token. entailer!. repeat right. split; auto.
                         ** entailer.
                     ++ Intros ab0. forward. Exists (fst ab). unfold my_kalloc_token. rewrite mem_mgr_split. 
-                        Exists (fst ab) (snd ab). if_tac; auto_contradict. Exists (fst ab0) (snd ab0). rewrite mem_mgr_split; entailer!.
+                        Exists (fst ab) (snd ab). if_tac_auto_contradict. Exists (fst ab0) (snd ab0). rewrite mem_mgr_split; entailer!.
                         repeat right; split; auto.
--if_tac; auto_contradict. unfold KF_globals. entailer!.
+-if_tac_auto_contradict. unfold KF_globals. entailer!.
 - forward_call (kalloc_spec_sub KF_APD t_run) (gv, sh , ls, xx, original_freelist_pointer). (* kalloc *)
-+ if_tac; auto_contradict. entailer!.
-+ if_tac; auto_contradict. 
++ if_tac_auto_contradict. entailer!.
++ if_tac_auto_contradict. 
     * forward_call (kfree_spec_sub KF_APD t_run) (pa2, gv, sh , ls, xx, original_freelist_pointer). (* call kfree *)
-        -- if_tac; auto_contradict. unfold my_kalloc_token. entailer!.
-        -- if_tac; auto_contradict. forward_call (kalloc_spec_sub KF_APD t_run) (gv, sh , (original_freelist_pointer :: ls), xx, pa2). (* kalloc *)
+        -- if_tac_auto_contradict. unfold my_kalloc_token. entailer!.
+        -- if_tac_auto_contradict. forward_call (kalloc_spec_sub KF_APD t_run) (gv, sh , (original_freelist_pointer :: ls), xx, pa2). (* kalloc *)
             if_tac.
                 ++ forward.
                 ++ Intros ab. destruct ls; auto_contradict;
@@ -491,35 +546,80 @@ forward_call (kfree_spec_sub KF_APD t_run) (pa1, gv, sh , ls, xx, original_freel
                     do 4 right; left; split; auto.
     * Intros ab. destruct ls; auto_contradict.  
     forward_call (kfree_spec_sub KF_APD t_run) (pa2, gv, sh , snd ab, xx, fst ab). (* call kfree *)
-        -- if_tac; auto_contradict. unfold my_kalloc_token at 2. rewrite kalloc_token_sz_split. entailer!.
-        -- if_tac; auto_contradict. rewrite mem_mgr_split. Intros. forward_call (kalloc_spec_sub KF_APD t_run) (gv, sh , fst ab::snd ab, xx, pa2). (* kalloc *)
+        -- if_tac_auto_contradict. unfold my_kalloc_token at 2. rewrite kalloc_token_sz_split. entailer!.
+        -- if_tac_auto_contradict. rewrite mem_mgr_split. Intros. forward_call (kalloc_spec_sub KF_APD t_run) (gv, sh , fst ab::snd ab, xx, pa2). (* kalloc *)
             ++ unfold my_kalloc_token. rewrite mem_mgr_split.  entailer!.
-            ++ forward. if_tac; auto_contradict. Intros ab0. Exists pa2 (fst ab0) (snd ab0). rewrite mem_mgr_split. unfold KF_globals, my_kalloc_token. rewrite mem_mgr_split. entailer!.
+            ++ forward. if_tac_auto_contradict. Intros ab0. Exists pa2 (fst ab0) (snd ab0). rewrite mem_mgr_split. unfold KF_globals, my_kalloc_token. rewrite mem_mgr_split. entailer!.
                do 4 right. left; split; auto.
-- if_tac; auto_contradict. unfold KF_globals. rewrite kalloc_token_sz_split. unfold my_kalloc_token. rewrite kalloc_token_sz_split. entailer!.
-- if_tac; auto_contradict.
+- if_tac_auto_contradict. unfold KF_globals. rewrite kalloc_token_sz_split. unfold my_kalloc_token. rewrite kalloc_token_sz_split. entailer!.
+- if_tac_auto_contradict.
     forward_call (kalloc_spec_sub KF_APD t_run) (gv, sh , original_freelist_pointer::ls, xx, pa1). (* kalloc *)
-    if_tac; auto_contradict.
+    if_tac_auto_contradict.
     Intros ab.
     forward_call (kfree_spec_sub KF_APD t_run) (pa2, gv, sh , snd ab, xx, fst ab). (* call kfree *)
     ++ entailer!.
-    ++ if_tac; auto_contradict. forward_call (kalloc_spec_sub KF_APD t_run) (gv, sh , snd ab, xx, fst ab). (* kalloc *)
-        forward. if_tac; auto_contradict; inversion H5.
-        ** Exists (fst ab). if_tac; auto_contradict.
+    ++ if_tac_auto_contradict. forward_call (kalloc_spec_sub KF_APD t_run) (gv, sh , snd ab, xx, fst ab). (* kalloc *)
+        forward. if_tac_auto_contradict; inversion H5.
+        ** Exists (fst ab). if_tac_auto_contradict.
         unfold my_kalloc_token, KF_globals. entailer!.
         do 2 right; left; split; auto.
-        ** Intros ab0. Exists (fst ab). if_tac; auto_contradict.
+        ** Intros ab0. Exists (fst ab). if_tac_auto_contradict.
             Exists (fst ab0) (snd ab0). unfold my_kalloc_token, KF_globals. entailer!.
             do 3 right; left; split; auto.
-- if_tac; auto_contradict. unfold KF_globals. unfold my_kalloc_token. entailer!.
-- if_tac; auto_contradict. forward_call (kalloc_spec_sub KF_APD t_run) (gv, sh , original_freelist_pointer::ls, xx, pa1). (* kalloc *)
-    if_tac; auto_contradict.
+- if_tac_auto_contradict. unfold KF_globals. unfold my_kalloc_token. entailer!.
+- if_tac_auto_contradict. forward_call (kalloc_spec_sub KF_APD t_run) (gv, sh , original_freelist_pointer::ls, xx, pa1). (* kalloc *)
+    if_tac_auto_contradict.
     Intros ab.
     forward_call (kfree_spec_sub KF_APD t_run) (pa2, gv, sh , snd ab, xx, fst ab). (* call kfree *)
-    + if_tac; auto_contradict. unfold my_kalloc_token at 2; entailer!.
-    + if_tac; auto_contradict.
+    + if_tac_auto_contradict. unfold my_kalloc_token at 2; entailer!.
+    + if_tac_auto_contradict.
     forward_call (kalloc_spec_sub KF_APD t_run) (gv, sh , fst ab::snd ab, xx, pa2). (* kalloc *)
-    if_tac; auto_contradict.
+    if_tac_auto_contradict.
     Intros ab0. forward. Exists pa2. unfold KF_globals. unfold my_kalloc_token; entailer!.
     inversion H8. rewrite H14, H15. inversion H5. rewrite H16, H17. entailer!.
-Qed. 
+Qed.
+
+Lemma body_kfree_kfree_kalloc: semax_body KFVprog KFGprog f_kfree_kfree_kalloc kfree_kfree_kalloc_spec.
+Proof.
+start_function.
+Intros.
+if_tac; if_tac; destruct H; 
+forward_call (kfree_spec_sub KF_APD t_run) (pa1, gv, sh , ls, xx, original_freelist_pointer). (* call kfree *)
+- if_tac_auto_contradict. unfold KF_globals. entailer!.
+- if_tac_auto_contradict;
+    forward_call (kfree_spec_sub KF_APD t_run) (pa2, gv, sh , ls, xx, original_freelist_pointer). (* call kfree*)
+    + if_tac_auto_contradict. entailer!.
+    + if_tac_auto_contradict.
+        forward_call (kalloc_spec_sub KF_APD t_run) (gv, sh , ls, xx, original_freelist_pointer). (* kalloc *)
+        if_tac_auto_contradict. 
+        * forward. Exists nullval. unfold KF_globals. entailer!.
+        * forward. Exists original_freelist_pointer. Exists (fst ab) (snd ab). entailer!. 
+        unfold my_kalloc_token, KF_globals. entailer!.
+-if_tac_auto_contradict. unfold KF_globals. entailer!.
+-if_tac_auto_contradict;
+forward_call (kfree_spec_sub KF_APD t_run) (pa2, gv, sh , ls, xx,original_freelist_pointer). (* call kfree*)
++ if_tac_auto_contradict. entailer!. unfold my_kalloc_token; entailer!. 
++ if_tac_auto_contradict.
+    forward_call (kalloc_spec_sub KF_APD t_run) (gv, sh , original_freelist_pointer::ls, xx, pa2). (* kalloc *)
+    if_tac_auto_contradict. 
+    forward. Exists pa2. unfold KF_globals. entailer!.
+        * do 3 right. split; auto.
+        * unfold my_kalloc_token. entailer!. inversion H0. rewrite H9, H10. entailer.
+- if_tac_auto_contradict. unfold KF_globals, my_kalloc_token. entailer!.
+- if_tac_auto_contradict. 
+forward_call (kfree_spec_sub KF_APD t_run) (pa2, gv, sh , original_freelist_pointer::ls, xx,pa1). (* call kfree*)
++ if_tac_auto_contradict. entailer!.
++ if_tac_auto_contradict. forward_call (kalloc_spec_sub KF_APD t_run) (gv, sh , original_freelist_pointer::ls, xx, pa1). (* kalloc *)
+    if_tac_auto_contradict.
+    Intros ab. forward. Exists pa1. unfold my_kalloc_token, KF_globals. entailer!.
+    * do 2 right; left; split; auto.
+    * inversion H6. rewrite H9, H10. entailer.
+- if_tac_auto_contradict. unfold my_kalloc_token, KF_globals. entailer!.
+- if_tac_auto_contradict. forward_call (kfree_spec_sub KF_APD t_run) (pa2, gv, sh , original_freelist_pointer::ls, xx,pa1). (* call kfree*)
+    + if_tac_auto_contradict. unfold my_kalloc_token. entailer!.
+    + if_tac_auto_contradict. forward_call (kalloc_spec_sub KF_APD t_run) (gv, sh , pa1::original_freelist_pointer::ls, xx, pa2). (* kalloc *)
+    if_tac_auto_contradict. Intros ab.
+    forward. Exists pa2. unfold KF_globals, my_kalloc_token. entailer!.
+    inversion H6.
+    entailer.
+Qed.
