kalloc/tactics.v
@@ -4,4 +4,8 @@ Require Import VST.floyd.proofauto.
 
 Ltac auto_contradict := try discriminate; try contradiction.
 
+Ltac if_tac_auto_contradict :=
+  if_tac; auto_contradict.
+
+
 Definition PGSIZE : Z := 4096.
